scheduler/SchIAproof.v
@@ -276,7 +276,7 @@ Section SchIA.
     steps_r. hss. steps_r.
     by_coind "CIH". iFrame.
     Unshelve. all: ss.
-  (*SLOW*)Admitted.
+  (*SLOW*)Qed.
 
   Lemma simF_spawn :
     HSim.sim_fun open SchAMod SchIMod SchA.init_cond Ist (Some SchHdr.spawn).
@@ -342,7 +342,7 @@ Section SchIA.
     force_l (nths ↑). force_l.
     iSplitL "tid TKNQ0 WI"; iFrame; eauto.
     step. iFrame. iSplit; eauto. iExists _, _, _. esplits; eauto.
-  (*SLOW*)Admitted.
+  (*SLOW*)Qed.
 
   Lemma simF_yield :
     HSim.sim_fun open SchAMod SchIMod SchA.init_cond Ist (Some SchHdr.yield).
@@ -376,7 +376,7 @@ Section SchIA.
     force_l (tt↑). steps_l. steps_r.
     force_l. iSplitL "tid WI". { iFrame. eauto. }
     step. iFrame. iSplit; eauto. iExists _, _, _. iSplit; eauto.
-  (*SLOW*)Admitted.
+  (*SLOW*)Qed.
 
   Lemma simF_join :
     HSim.sim_fun open SchAMod SchIMod SchA.init_cond Ist (Some SchHdr.join).
@@ -476,7 +476,7 @@ Section SchIA.
       eapply fragree_incl_false. et.
     }
   Unshelve. all : ss.
-  (*SLOW*)Admitted.
+  (*SLOW*)Qed.
 
   Lemma simF_get_tid :
     HSim.sim_fun open SchAMod SchIMod SchA.init_cond Ist (Some SchHdr.get_tid).
@@ -490,7 +490,7 @@ Section SchIA.
     iPoseProof (tid_admin_some_user with "[TA tid]") as "%"; iFrame; subst.
     steps_r. forces_l. iSplitL "tid"; eauto.
     step. iSplit; eauto. iFrame. iExists _, _, _. iSplit; eauto.
-  (*SLOW*)Admitted.
+  (*SLOW*)Qed.
 
   Lemma sim : HSim.t open SchAMod SchIMod SchA.init_cond Ist.
   Proof using FunInSp SchInSp.
